LambdaLet.v
@@ -1,17 +1,18 @@
 From mathcomp Require Import all_ssreflect.
 Require Import Util.
 
+Definition ctor := nat.
+
 Inductive term : Type :=
   | Var of nat
   | Loc of nat
   | Abs of term
   | App of term & term
-  | Let of seq term & term.
+  | Let of seq term & term
+  | Ctor of ctor & seq term
+  | Case of term & seq (ctor * nat * term).
 
-Inductive value : term -> Prop :=
-  | value_abs t : value (Abs t).
-
-Hint Constructors value.
+(* まず，まともな帰納法の原理を得る *)
 
 Definition term_rect'
   (P : term -> Type)
@@ -19,7 +20,9 @@ Definition term_rect'
   (HLoc : forall l, P (Loc l))
   (HAbs : forall t, P t -> P (Abs t))
   (HApp : forall t1, P t1 -> forall t2, P t2 -> P (App t1 t2))
-  (HLet : forall ts, foldr (fun t => prod (P t)) unit ts -> forall t, P t -> P (Let ts t)) :=
+  (HLet : forall ts, foldr (fun t => prod (P t)) unit ts -> forall t, P t -> P (Let ts t))
+  (HCtor : forall c ts, foldr (fun t => prod (P t)) unit ts -> P (Ctor c ts))
+  (HCase : forall t, P t -> forall pts, foldr (fun pt => prod (P pt.2)) unit pts -> P (Case t pts)) :=
   fix term_ind t :=
     match t as t0 return P t0 with
     | Var _ => HVar _
@@ -31,39 +34,75 @@ Definition term_rect'
         | nil => tt
         | t :: ts => pair (term_ind t) (term_ind' ts)
         end) ts) _ (term_ind t)
+    | Ctor c ts => HCtor _ _ ((fix term_ind' ts :=
+        match ts as ts0 return foldr (fun t => prod (P t)) unit ts0 with
+        | nil => tt
+        | t :: ts => pair (term_ind t) (term_ind' ts)
+        end) ts)
+    | Case t pts => HCase _ (term_ind t) _ ((fix term_ind' pts :=
+        match pts as pts0 return foldr (fun pt => prod (P pt.2)) unit pts0 with
+        | nil => tt
+        | (_, _, t) :: ts => pair (term_ind t) (term_ind' ts)
+        end) pts)
     end.
 
-Fixpoint encode t :=
-  match t with
-  | Var x => GenTree.Leaf (inl x)
-  | Loc l => GenTree.Leaf (inr l)
-  | Abs t => GenTree.Node 0 [:: encode t]
-  | App t1 t2 => GenTree.Node 1 [:: encode t1; encode t2]
-  | Let ts t =>  GenTree.Node 2 (encode t :: map encode ts)
-  end.
+Lemma sumbool_cast {A B C D : Prop} :
+  (A -> C) ->
+  (B -> D) ->
+  { A } + { B } ->
+  { C } + { D }.
+Proof. by move => HL HR [ /HL | /HR ] ?; [ left | right ]. Qed.
 
-Fixpoint decode t :=
-  match t with
-  | GenTree.Leaf (inl x) => Some (Var x)
-  | GenTree.Leaf (inr l) => Some (Loc l)
-  | GenTree.Node 0 [:: t'] => omap Abs (decode t')
-  | GenTree.Node 1 [:: t1'; t2'] =>
-      if decode t1' is Some t1 then omap (App t1) (decode t2')
-      else None
-  | GenTree.Node 2 (t' :: ts') => omap (Let (pmap decode ts')) (decode t')
-  | GenTree.Node _ _ => None
-  end.
-
-Lemma codeK : pcancel encode decode.
+Definition term_eq_dec : forall (t t' : term), { t = t' } + { t <> t' }.
 Proof.
-  elim /term_rect' =>
-    /= [ | | ? -> | ? -> ? -> | ts IHts t -> ] //=.
-  congr (Some (Let _ t)).
-  elim: ts IHts => /= [ | ? ? IHIH [ -> ? ] ] //=.
-  by rewrite IHIH.
-Qed.
+  refine (fix term_eq_dec t t' :=
+    match t, t' return { t = t' } + { t <> t' } with
+    | Var x, Var y => sumbool_cast _ _ (PeanoNat.Nat.eq_dec x y)
+    | Loc l, Loc l' => sumbool_cast _ _ (PeanoNat.Nat.eq_dec l l')
+    | Abs t, Abs t' => sumbool_cast _ _ (term_eq_dec t t')
+    | App t11 t12, App t21 t22 =>
+        sumbool_cast _ _
+          (Sumbool.sumbool_and _ _ _ _
+             (term_eq_dec t11 t21) (term_eq_dec t12 t22))
+    | Let t11s t12, Let t21s t22 =>
+        sumbool_cast _ _
+          (Sumbool.sumbool_and _ _ _ _
+            (List.list_eq_dec term_eq_dec t11s t21s)
+            (term_eq_dec t12 t22))
+    | Ctor c ts, Ctor c' ts' =>
+        sumbool_cast _ _
+          (Sumbool.sumbool_and _ _ _ _
+            (PeanoNat.Nat.eq_dec c c')
+            (List.list_eq_dec term_eq_dec ts ts'))
+    | Case t pts, Case t' pts' =>
+        sumbool_cast _ _
+          (Sumbool.sumbool_and _ _ _ _
+            (term_eq_dec t t')
+            (List.list_eq_dec (fun pt pt' =>
+              match pt, pt' with
+              | ((c, n), t), ((c', n'), t') =>
+                  sumbool_cast _ _
+                    (Sumbool.sumbool_and _ _ _ _
+                      (PeanoNat.Nat.eq_dec c c')
+                      (Sumbool.sumbool_and _ _ _ _
+                        (PeanoNat.Nat.eq_dec n n')
+                        (term_eq_dec t t')))
+              end) pts pts'))
+    | _, _ => right _
+    end);
+  repeat match goal with
+  | |- _ /\ _ -> _ => move => [ ]
+  | |- _ \/ _ -> _ => move => [ ]
+  | |- _ = _ -> _ => move => ->
+  | |- _ <> _ -> _ => move => ?
+  | |- _ <> _ => inversion 1
+  end; eauto.
+Defined.
 
-Definition term_eqMixin := PcanEqMixin codeK.
+Lemma term_eqP : Equality.axiom term_eq_dec.
+Proof. move => t t'. by case (term_eq_dec t t') => ?; [ left | right ]. Qed.
+
+Definition term_eqMixin := EqMixin term_eqP.
 Canonical term_eqType := Eval hnf in EqType _ term_eqMixin.
 
 Definition term_ind'
@@ -73,15 +112,30 @@ Definition term_ind'
   (HAbs : forall t, P t -> P (Abs t))
   (HApp : forall t1, P t1 -> forall t2, P t2 -> P (App t1 t2))
   (HLet : forall ts, { in ts, forall t, P t } -> forall t, P t -> P (Let ts t))
+  (HCtor : forall c ts, { in ts, forall t, P t } -> P (Ctor c ts))
+  (HCase : forall t, P t ->
+    forall pts, (forall c n t, (c, n, t) \in pts -> P t) -> P (Case t pts))
   : forall t, P t.
 Proof.
-  elim /term_rect' => [ | | | | ts IHts ] //=.
-  apply: HLet.
-  elim: ts IHts => /= [ ? ? | ? ? IHts [ ? ? ] ? ].
-  - by rewrite in_nil.
-  - rewrite in_cons => /orP [ /eqP -> // | ].
-    exact: IHts.
+  elim /term_rect' => [ | | | | ts IHts | ? ts IHts | ? ? pts IHpts ] //=.
+  - apply: HLet.
+    elim: ts IHts => /= [ ? ? | ? ? IHts [ ? ? ] ? ].
+    + by rewrite in_nil.
+    + rewrite in_cons => /orP [ /eqP -> // | ].
+      exact: IHts.
+  - apply: HCtor.
+    elim: ts IHts => /= [ ? ? | ? ? IHts [ ? ? ] ? ].
+    + by rewrite in_nil.
+    + rewrite in_cons => /orP [ /eqP -> // | ].
+      exact: IHts.
+  - apply: HCase => //.
+    elim: pts IHpts => /= [ ? ? ? ? | [ [ ? ? ] ? ] ? IHpts /= [ ? ? ] ? ? ? ].
+    + by rewrite in_nil.
+    + rewrite in_cons => /orP [ /andP /= [ ? /eqP -> ] // | ].
+      exact: IHpts.
 Qed.
+
+(* シフトや代入の定義と，それらについての補題を証明する *)
 
 Fixpoint rename_term r t :=
   match t with
@@ -92,6 +146,10 @@ Fixpoint rename_term r t :=
   | Let ts t =>
       let r' := upnren r (size ts) in
       Let (map (rename_term r') ts) (rename_term r' t)
+  | Ctor c ts => Ctor c (map (rename_term r) ts)
+  | Case t pts =>
+      Case (rename_term r t)
+        (map (fun pt => (pt.1, rename_term (upnren r (pt.1.2)) pt.2)) pts)
   end.
 
 Program Instance RenameTerm : Rename term :=
@@ -99,21 +157,30 @@ Program Instance RenameTerm : Rename term :=
 Next Obligation.
   elim /term_ind' : t r r' H => /=;
   intros; f_equal; eauto using eq_upren, eq_upnren.
-  by apply /eq_in_map => ? /H; eauto using eq_upnren.
+  - by apply /eq_in_map => ? /H; eauto using eq_upnren.
+  - by apply /eq_in_map => ? /H; eauto using eq_upnren.
+  - apply /eq_in_map => [ [ [ ? ? ] ? ] /= /H0 ? ].
+    f_equal. eauto using eq_upnren.
 Qed.
 
 Program Instance RenameLemmasTerm : RenameLemmas term.
 Next Obligation.
   induction t using term_ind' => /=; f_equal;
   eauto using rename_id_upren, rename_id_upnren.
-  apply map_id_in => ? /H. eauto using rename_id_upnren.
+  - apply map_id_in => ? /H. eauto using rename_id_upnren.
+  - apply map_id_in => ? /H. eauto using rename_id_upnren.
+  - apply: map_id_in => [ [ [ ? ? ] ? ] /= /H ? ].
+    f_equal. eauto using rename_id_upnren.
 Qed.
 Next Obligation.
-  elim /term_ind' : t r r' => /=; intros; f_equal; rewrite ?size_map;
+  elim /term_ind' : t r r' => /=; intros; f_equal; rewrite ?size_map -?map_comp;
   eauto using rename_rename_comp_upren, rename_rename_comp_upnren.
-  rewrite -map_comp.
-  apply /eq_in_map => ? /H.
-  eauto using rename_rename_comp_upnren.
+  - apply /eq_in_map => ? /H.
+    eauto using rename_rename_comp_upnren.
+  - apply /eq_in_map => ? /H.
+    eauto using rename_rename_comp_upnren.
+  - apply /eq_in_map => [ [ [ ? ? ] ? ] /= /H0 ? ].
+    f_equal. eauto using rename_rename_comp_upnren.
 Qed.
 
 Fixpoint subst_term s t :=
@@ -125,46 +192,68 @@ Fixpoint subst_term s t :=
   | Let ts t =>
       let s' := upn s (size ts) in
       Let (map (subst_term s') ts) (subst_term s' t)
+  | Ctor c ts => Ctor c (map (subst_term s) ts)
+  | Case t pts =>
+      Case (subst_term s t)
+        (map (fun pt => (pt.1, subst_term (upn s (pt.1.2)) pt.2)) pts)
   end.
 
 Program Instance SubstTerm : Subst term := { subst := subst_term }.
 Next Obligation.
   elim /term_ind' : t s s' H => /=; intros; f_equal;
   eauto using eq_up, eq_upn.
-  apply /eq_in_map => ? /H; eauto using eq_upn.
+  - apply /eq_in_map => ? /H; eauto using eq_upn.
+  - apply /eq_in_map => ? /H; eauto using eq_upn.
+  - apply /eq_in_map => [ [ [ ? ? ] ? ] /= /H0 ? ].
+    f_equal. eauto using eq_upn.
 Qed.
 
 Program Instance SubstLemmasTerm : SubstLemmas term.
 Next Obligation.
   elim /term_ind' : t => /=; intros; f_equal;
   eauto using subst_id_up, subst_id_upn.
-  apply: map_id_in => ? /H. eauto using subst_id_upn.
+  - apply: map_id_in => ? /H. eauto using subst_id_upn.
+  - apply: map_id_in => ? /H. eauto using subst_id_upn.
+  - apply: map_id_in => [ [ [ ? ? ] ? ] /= /H0 ? ].
+    f_equal. eauto using subst_id_upn.
 Qed.
 Next Obligation.
   elim /term_ind' : t r => /=; intros; f_equal;
   eauto using rename_subst_up, rename_subst_upn.
-  apply /eq_in_map => ? /H. eauto using rename_subst_upn.
+  - apply /eq_in_map => ? /H. eauto using rename_subst_upn.
+  - apply /eq_in_map => ? /H. eauto using rename_subst_upn.
+  - apply /eq_in_map => [ [ [ ? ? ] ? ] /= /H0 ? ].
+    f_equal. eauto using rename_subst_upn.
 Qed.
 Next Obligation.
-  elim /term_ind' : t r s => /=; intros; f_equal; rewrite ?size_map;
+  elim /term_ind' : t r s => /=; intros; f_equal; rewrite ?size_map -?map_comp;
   eauto using subst_rename_comp_up, subst_rename_comp_upn.
-  rewrite -map_comp.
-  apply /eq_in_map => ? /H.
-  eauto using subst_rename_comp_upn.
+  - apply /eq_in_map => ? /H.
+    eauto using subst_rename_comp_upn.
+  - apply /eq_in_map => ? /H.
+    eauto using subst_rename_comp_upn.
+  - apply /eq_in_map => [ [ [ ? ? ] ? ] /= /H0 ? ].
+    f_equal. eauto using subst_rename_comp_upn.
 Qed.
 Next Obligation.
-  elim /term_ind' : t r s => /=; intros; f_equal; rewrite ?size_map;
+  elim /term_ind' : t r s => /=; intros; f_equal; rewrite ?size_map -?map_comp;
   eauto using rename_subst_comp_up, rename_subst_comp_upn.
-  rewrite -map_comp.
-  apply /eq_in_map => ? /H.
-  eauto using rename_subst_comp_upn.
+  - apply /eq_in_map => ? /H.
+    eauto using rename_subst_comp_upn.
+  - apply /eq_in_map => ? /H.
+    eauto using rename_subst_comp_upn.
+  - apply /eq_in_map => [ [ [ ? ? ] ? ] /= /H0 ? ].
+    f_equal. eauto using rename_subst_comp_upn.
 Qed.
 
 Program Instance SubstLemmas'Term : SubstLemmas' term.
 Next Obligation.
-  elim /term_ind' : t s s' => /=; intros; f_equal; rewrite ?size_map;
+  elim /term_ind' : t s s' => /=; intros; f_equal; rewrite ?size_map -?map_comp;
   eauto using subst_subst_comp_up, subst_subst_comp_upn.
-  rewrite -map_comp.
-  apply /eq_in_map => ? /H.
-  eauto using subst_subst_comp_upn.
+  - apply /eq_in_map => ? /H.
+    eauto using subst_subst_comp_upn.
+  - apply /eq_in_map => ? /H.
+    eauto using subst_subst_comp_upn.
+  - apply /eq_in_map => [ [ [ ? ? ] ? ] /= /H0 ? ].
+    f_equal. eauto using subst_subst_comp_upn.
 Qed.
